src/program_proof/tulip/program/util/decode_value.v
@@ -1,0 +1,59 @@
+From Perennial.program_proof.tulip.program Require Import prelude.
+From Perennial.program_proof.tulip.program.util Require Import decode_string.
+From Perennial.program_proof Require Import marshal_stateless_proof.
+
+Opaque encode_string.
+
+Section program.
+  Context `{!heapGS Σ, !paxos_ghostG Σ}.
+
+  Theorem wp_DecodeValue (bsP : Slice.t) (v : dbval) (bstail : list u8) :
+    {{{ own_slice_small bsP byteT (DfracOwn 1) (encode_dbval v ++ bstail) }}}
+      DecodeValue (to_val bsP)
+    {{{ (dataP : Slice.t), RET (dbval_to_val v, (to_val dataP));
+        own_slice_small dataP byteT (DfracOwn 1) bstail
+    }}}.
+  Proof.
+    iIntros (Φ) "Hbs HΦ".
+    wp_rec.
+
+    (*@ func DecodeValue(bs []byte) (tulip.Value, []byte) {                     @*)
+    (*@     b, bs1 := marshal.ReadBool(bs)                                      @*)
+    (*@                                                                         @*)
+
+    (*@     if !b {                                                             @*)
+    (*@         v := tulip.Value{                                               @*)
+    (*@             Present : false,                                            @*)
+    (*@             Content : "",                                               @*)
+    (*@         }                                                               @*)
+    (*@         return v, bs1                                                   @*)
+    (*@     }                                                                   @*)
+    (*@                                                                         @*)
+    destruct v as [s |]; wp_pures; last first.
+    { wp_apply (wp_ReadBool with "Hbs").
+      iIntros (b bs1) "[%Hb Hbs]".
+      replace (uint.Z (W8 0)) with 0 in Hb; last word.
+      simpl in Hb. subst b.
+      wp_pures.
+      by iApply "HΦ".
+    }
+
+    (*@     s, data := DecodeString(bs1)                                        @*)
+    (*@     v := tulip.Value{                                                   @*)
+    (*@         Present : true,                                                 @*)
+    (*@         Content : s,                                                    @*)
+    (*@     }                                                                   @*)
+    (*@     return v, data                                                      @*)
+    (*@ }                                                                       @*)
+    simpl.
+    wp_apply (wp_ReadBool with "Hbs").
+    iIntros (b bs1) "[%Hb Hbs]".
+    replace (uint.Z (W8 1)) with 1 in Hb; last word.
+    simpl in Hb. subst b.
+    wp_apply (wp_DecodeString with "Hbs").
+    iIntros (dataP) "Hdata".
+    wp_pures.
+    by iApply "HΦ".
+  Qed.
+
+End program.
