src/program_proof/tulip/program/util/decode_write_entry.v
@@ -1,0 +1,36 @@
+From Perennial.program_proof.tulip.program Require Import prelude.
+From Perennial.program_proof.tulip.program.util Require Import decode_string decode_value.
+From Perennial.program_proof Require Import marshal_stateless_proof.
+
+Section program.
+  Context `{!heapGS Σ, !paxos_ghostG Σ}.
+
+  Theorem wp_DecodeWriteEntry (bsP : Slice.t) (x : dbmod) (bstail : list u8) :
+    {{{ own_slice_small bsP byteT (DfracOwn 1) (encode_dbmod x ++ bstail) }}}
+      DecodeWriteEntry (to_val bsP)
+    {{{ (dataP : Slice.t), RET (dbmod_to_val x, (to_val dataP));
+        own_slice_small dataP byteT (DfracOwn 1) bstail
+    }}}.
+  Proof.
+    iIntros (Φ) "Hbs HΦ".
+    wp_rec.
+
+    (*@ func DecodeWriteEntry(bs []byte) (tulip.WriteEntry, []byte) {           @*)
+    (*@     k, bs1 := DecodeString(bs)                                          @*)
+    (*@     v, data := DecodeValue(bs1)                                         @*)
+    (*@     x := tulip.WriteEntry{                                              @*)
+    (*@         Key   : k,                                                      @*)
+    (*@         Value : v,                                                      @*)
+    (*@     }                                                                   @*)
+    (*@     return x, data                                                      @*)
+    (*@ }                                                                       @*)
+    rewrite /encode_dbmod -app_assoc.
+    wp_apply (wp_DecodeString with "Hbs").
+    iIntros (bs1P) "Hbs".
+    wp_apply (wp_DecodeValue with "Hbs").
+    iIntros (dataP) "Hdata".
+    wp_pures.
+    by iApply "HΦ".
+  Qed.
+
+End program.
