src/program_proof/tulip/program/util/encode_value.v
@@ -1,0 +1,44 @@
+From Perennial.program_proof.tulip.program Require Import prelude.
+From Perennial.program_proof.tulip.program.util Require Import encode_string.
+From Perennial.program_proof Require Import marshal_stateless_proof.
+
+Section program.
+  Context `{!heapGS Σ, !paxos_ghostG Σ}.
+
+  Theorem wp_EncodeValue (bsP : Slice.t) (v : dbval) (bs : list u8) :
+    {{{ own_slice bsP byteT (DfracOwn 1) bs }}}
+      EncodeValue (to_val bsP) (dbval_to_val v)
+    {{{ (dataP : Slice.t), RET (to_val dataP);
+        own_slice dataP byteT (DfracOwn 1) (bs ++ encode_dbval v)
+    }}}.
+  Proof.
+    iIntros (Φ) "Hbs HΦ".
+    wp_rec.
+
+    (*@ func EncodeValue(bs []byte, v tulip.Value) []byte {                     @*)
+    (*@     if !v.Present {                                                     @*)
+    (*@         data := marshal.WriteBool(bs, false)                            @*)
+    (*@         return data                                                     @*)
+    (*@     }                                                                   @*)
+    (*@                                                                         @*)
+    destruct v as [s |]; last first.
+    { wp_apply (wp_WriteBool with "Hbs").
+      iIntros (p1) "Hp1".
+      wp_pures.
+      by iApply "HΦ".
+    }
+
+    (*@     bs1 := marshal.WriteBool(bs, true)                                  @*)
+    (*@     data := EncodeString(bs1, v.Content)                                @*)
+    (*@     return data                                                         @*)
+    (*@ }                                                                       @*)
+    wp_apply (wp_WriteBool with "Hbs").
+    iIntros (p1) "Hp1".
+    wp_apply (wp_EncodeString with "Hp1").
+    iIntros (p2) "Hp2".
+    wp_pures.
+    iApply "HΦ".
+    by rewrite -app_assoc.
+  Qed.
+
+End program.
