src/program_proof/tulip/program/util/encode_write_entry.v
@@ -1,0 +1,32 @@
+From Perennial.program_proof.tulip.program Require Import prelude.
+From Perennial.program_proof.tulip.program.util Require Import encode_string encode_value.
+From Perennial.program_proof Require Import marshal_stateless_proof.
+
+Section program.
+  Context `{!heapGS Σ, !paxos_ghostG Σ}.
+
+  Theorem wp_EncodeWriteEntry (bsP : Slice.t) (x : dbmod) (bs : list u8) :
+    {{{ own_slice bsP byteT (DfracOwn 1) bs }}}
+      EncodeWriteEntry (to_val bsP) (dbmod_to_val x)
+    {{{ (dataP : Slice.t), RET (to_val dataP);
+        own_slice dataP byteT (DfracOwn 1) (bs ++ encode_dbmod x)
+    }}}.
+  Proof.
+    iIntros (Φ) "Hbs HΦ".
+    wp_rec.
+
+    (*@ func EncodeWriteEntry(bs []byte, x tulip.WriteEntry) []byte {           @*)
+    (*@     bs1 := EncodeString(bs, x.Key)                                      @*)
+    (*@     data := EncodeValue(bs1, x.Value)                                   @*)
+    (*@     return data                                                         @*)
+    (*@ }                                                                       @*)
+    wp_apply (wp_EncodeString with "Hbs").
+    iIntros (p1) "Hbs".
+    wp_apply (wp_EncodeValue with "Hbs").
+    iIntros (dataP) "Hdata".
+    wp_pures.
+    rewrite -app_assoc.
+    by iApply "HΦ".
+  Qed.
+
+End program.
